rocq-osiris/theories/program_logic/pure/binding_rules.v
@@ -3,58 +3,58 @@ From osiris Require Import base.
 From osiris.lang Require Import lang ind.
 From osiris.semantics Require Import semantics.
 
-From osiris.program_logic.pure Require Import wp judgements pattern_rules.
+From osiris.program_logic.pure Require Import wp pure_rules judgements pattern_rules.
 
 (* A judgement for the evaluation of let bindings. *)
 
 Definition bindings η bs (φ : env -> Prop) (ψ : exn -> Prop) :=
-  pure_wp (eval_bindings η bs) φ ψ.
+  pure (eval_bindings η bs) φ ψ.
+
+Lemma pure_irrefutably_extend {E} η δ p v φ (ψ : E → Prop) :
+  pure (eval_pat η δ p v) φ ⊥ →
+  pure (irrefutably_extend η δ p v) φ ψ.
+Proof.
+  intros H.
+  apply pure_wp_try, (pure_wp_mono _ H);
+    firstorder eauto with pure.
+Qed.
 
 (* -------------------------------------------------------------------------- *)
 
 (* Syntax-directed reasoning rules for the auxiliary judgement [bindings]. *)
 
 Lemma bindings_cons_unary `{Encode A} η p e bs φ :
-  pure (eval η e)
-    (λ a : A,
-       pattern η [] p #a
-         (λ δ1, bindings η bs (λ δ2, φ (δ1 ++ δ2)) ⊥) False) ⊥ ->
+  pure (eval η e) (λ a : A, bindings η bs (λ η', pattern η η' p #a φ False) ⊥) ⊥ ->
   bindings η (Binding p e :: bs) φ ⊥.
 Proof.
   unfold bindings. simpl. intros He.
-  simpl_eval_bindings. apply pure_wp_bind.
-  apply pure_wp_Par_vals_left, pure_wp_bind.
-  apply (pure_wp_mono_ret _ He). intros v (a & -> & Ha).
-  apply pure_wp_widen_pat. unfold continue; simpl.
-  eapply pattern_env_mono. apply Ha. intros δ Hδ.
-  apply (pure_wp_mono_ret _ Hδ). intros η' Hη'.
-  apply pure_wp_ret, pure_wp_ret. apply Hη'.
+  simpl_eval_bindings. eapply pure_bind_unary.
+  eapply pure_par_seq; eauto.
+  eapply pure_ret_mono. { apply He. } intros a Ha.
+  eapply pure_ret_mono. { apply Ha. } intros η' Hpat.
+  apply pure_irrefutably_extend. apply Hpat.
 Qed.
 
-Lemma bindings_cons `{Encode A} η p e bs (φ1 : A -> Prop) φ P Q ψ :
+Lemma bindings_cons `{Encode A} η p e bs (φ1 : A -> Prop) φ2 φ ψ :
   pure (eval η e) φ1 ψ ->
-  (∀ (a : A), φ1 a -> pattern η [] p #a P False) ->
-  bindings η bs Q ψ ->
-  (∀ η δ, P η → Q δ → φ (η ++ δ)) →
+  bindings η bs φ2 ψ ->
+  (∀ (a : A) (η' : env), φ1 a -> φ2 η' -> pattern η η' p #a φ False) ->
   bindings η (Binding p e :: bs) φ ψ.
 Proof.
-  intros He Hp Hbs Hcov.
+  intros He Hbs Hp.
   unfold bindings.
-  simpl_eval_bindings. apply pure_wp_bind.
-  eapply pure_wp_Par_conseq; eauto.
-  - apply pure_wp_bind.
-    apply (pure_wp_mono_ret _ He). intros ? (? & -> & Hφ1).
-    apply pure_wp_widen_pat, Hp; auto.
-  - intros. unfold continue; simpl.
-    apply pure_wp_ret, pure_wp_ret. auto.
-  - intros exc Hexc. apply pure_wp_throw. tauto.
+  simpl_eval_bindings. eapply pure_bind_unary.
+  eapply pure_par; eauto.
+  intros a1 η' Hφ1 Hφ2.
+  apply pure_irrefutably_extend.
+  apply Hp; auto.
 Qed.
 
 Lemma bindings_nil η (φ : env -> Prop) ψ :
   φ [] ->
   bindings η [] φ ψ.
 Proof.
-  unfold bindings. simpl_eval_bindings. apply pure_wp_ret.
+  unfold bindings. simpl_eval_bindings. apply pure_ret. encode.
 Qed.
 
 Lemma bindings_var `{Encode A} η v e bs (φ : A -> Prop) φ' ψ :
@@ -67,22 +67,21 @@ Lemma bindings_var `{Encode A} η v e bs (φ : A -> Prop) φ' ψ :
 Proof.
   intros.
   eapply bindings_cons; eauto.
-  intros; unfold pattern.
-  eapply (pat_PVar _ _ _ _ (λ η, ∃ a, η = [(v,#a)] ∧ φ a)). eauto.
-  intros ?? (a & -> & Hφ) Hφ'. eauto.
+  intros; unfold pattern. simpl_eval_pat.
+  eapply pure_ret; eauto.
 Qed.
 
-Lemma bindings_pair `{Encode A, Encode B} η p1 p2 e bs φ
-  (φ1 : A -> Prop) (φ2 : B -> Prop) P Q ψ :
+Lemma bindings_pair `{Encode A, Encode B} η p1 p2 e bs φ φ'
+  (φ1 : A -> Prop) (φ2 : B -> Prop) ψ :
   pure (eval η e) (λ '(a, b), φ1 a /\ φ2 b) ψ ->
-  (∀ a b η', φ1 a -> φ2 b -> pattern η η' (PPair p1 p2) #(a, b) P False) ->
-  bindings η bs Q ψ ->
-  (∀ η δ, P η → Q δ → φ (η ++ δ)) →
+  bindings η bs φ' ψ ->
+  (∀ a b η', φ1 a -> φ2 b -> φ' η' -> pattern η η' (PPair p1 p2) #(a, b) φ False) ->
   bindings η (Binding (PPair p1 p2) e :: bs) φ ψ.
 Proof.
-  intros Hpure Hbs Hpat Hcov.
-  eapply (bindings_cons (A:=A*B)); eauto.
-  intros [a b] [Hψ1 Hψ2]. apply Hbs; auto.
+  intros Hpure Hbs Hpat.
+  eapply bindings_cons; eauto.
+  intros [a b] η' [Hψ1 Hψ2] Hη'.
+  auto.
 Qed.
 
 
@@ -94,55 +93,45 @@ Section eval_pat_app.
   Local Ltac rew := repeat (unfold orelse, try, glue2, continue || rewrite ?bind_as_try, ?try2_try2; simpl).
   Local Ltac ext x := let o := fresh "o" in f_equal; extensionality o; destruct o as [ x | ]; auto.
 
-  Local Open Scope stdpp.
-
-  Lemma eval_pat_app p v η δ :
-    eval_pat η δ p v = δ' ← eval_pat η [] p v; Some (δ' ++ δ).
+  Lemma eval_pat_app p v η δ : eval_pat η δ p v = 'δ' ← eval_pat η [] p v; ret (δ' ++ δ).
   Proof.
     revert p v δ.
     apply (pat_ind
-             (λ p, ∀ v δ, eval_pat η δ p v = mbind (λ δ', Some (δ' ++ δ)) (eval_pat η [] p v))
-             (λ ps, ∀ vs δ, eval_pats η δ ps vs = mbind (λ δ', Some (δ' ++ δ)) (eval_pats η [] ps vs) )
-             (λ fps, ∀ vs δ, pre_eval_fpats eval_pat η δ fps vs = mbind (λ δ', Some (δ' ++ δ)) (pre_eval_fpats eval_pat η [] fps vs))
+             (λ p, ∀ v δ, eval_pat η δ p v = bind (eval_pat η [] p v) (λ δ', ret (δ' ++ δ)))
+             (λ ps, ∀ vs δ, eval_pats η δ ps vs = bind (eval_pats η [] ps vs) (λ δ', ret (δ' ++ δ)))
+             (λ fps, ∀ vs δ, pre_eval_fpats eval_pat η δ fps vs = bind (pre_eval_fpats eval_pat η [] fps vs) (λ δ', ret (δ' ++ δ)))
           ); intros ? ?; intros; simpl_eval_pat || simpl_eval_pats || idtac; simpl; auto.
-    - rewrite IHp. destruct (eval_pat η [] p v0); auto.
-    - rewrite IHp1, IHp2. destruct (eval_pat η [] p1 v); simpl.
-      + rewrite !union_Some_l. reflexivity.
-      + rewrite !union_None_l. reflexivity.
+    - rewrite IHp. rewrite !bind_bind. reflexivity.
+    - rewrite IHp1, IHp2. rew. ext δ'.
     - destruct v; auto.
     - destruct v; auto. destruct (_ =? _)%string; auto.
-    - destruct v; auto. rewrite IHps.
-      destruct (lookup_path η π); simpl; auto.
-      destruct (val_as_loc_opt v0); simpl; auto.
-      destruct (locations.eqb _ _); auto.
+    - destruct v; auto. rewrite IHps. rew. ext l'. destruct (locations.eqb _ _); auto.
     - destruct v; auto.
     - destruct v; auto. destruct (int.eq _ _); auto.
     - destruct v; auto. destruct (_ =? _)%char; auto.
     - destruct v; auto. destruct (_ =? _)%string; auto.
     - destruct vs; auto.
-    - destruct vs; auto. rewrite IHp.
-      destruct (eval_pat η [] p v); simpl; last reflexivity.
-      rewrite !bind_with_Some.
-      rewrite (IHps _ (e ++ δ)).
-      rewrite (IHps _ e).
-      destruct (eval_pats η [] ps vs); simpl; auto.
-      by rewrite app_assoc.
-    - destruct (lookup_name vs f); simpl; auto.
-      rewrite IHp.
-      destruct (eval_pat η [] p v); simpl; auto.
-      rewrite IHfps.
-      rewrite (IHfps _ e).
-      destruct (pre_eval_fpats eval_pat η [] fps vs); simpl; auto.
-      by rewrite app_assoc.
+    - destruct vs; auto. rewrite IHp. rew. ext δ1. rew.
+      rewrite (IHps _ δ1), (IHps _ (δ1 ++ _)).
+      rew. ext δ2. rewrite app_assoc. auto.
+    - rew. ext v.
+      rewrite IHp. rew. ext δ1.
+      rewrite IHfps. rew.
+      rewrite (IHfps _ (δ1 ++ _)). rew.
+      ext δ2. rewrite app_assoc. auto.
   Qed.
 End eval_pat_app.
 
 Lemma pattern_app η δ p v φ ψ :
   pattern η δ p v φ ψ ↔ pattern η [] p v (λ δ', φ (δ' ++ δ)) ψ.
 Proof.
-  unfold pattern.
-  rewrite eval_pat_app.
-  destruct (eval_pat η [] p v); auto.
+  unfold pattern, pure.
+  rewrite eval_pat_app, <-pure_wp_reversible_bind.
+  apply pure_wp_ret_equiv; intros δ'.
+  rewrite <-pure_wp_reversible_ret. unfold returns.
+  split; intros (? & Heq & Hφ).
+  - exists δ'. rewrite Heq. eauto.
+  - exists (δ' ++ δ). simpl in Heq. rewrite <- Heq in Hφ. eauto.
 Qed.
 
 Definition binding `{Encode A} η p e φ ψ :=
@@ -156,8 +145,13 @@ Lemma binding_bindings_conseq `{Encode A} η p e bs (φ1 φ2 φ : env → Prop) 
 Proof.
   intros He Hbs Hp.
   eapply bindings_cons; eauto.
-  intros a Hpa. apply Hpa.
+  intros a η' Hpa Hη'.
+  apply pattern_app.
+  eapply pure_ret_mono. apply Hpa. eauto.
 Qed.
+
+Local Instance name : @ObserveInjective env env _.
+Proof. constructor. intros ??; simpl; auto. Qed.
 
 (* May be easier to use but assumes [e] cannot raise exceptions *)
 Lemma binding_bindings `{Encode A} η p e bs (φ1 φ2 φ : env → Prop) ψ :
@@ -166,15 +160,13 @@ Lemma binding_bindings `{Encode A} η p e bs (φ1 φ2 φ : env → Prop) ψ :
 Proof.
   intros He.
   unfold bindings.
-  simpl_eval_bindings. apply pure_wp_bind.
-  apply pure_wp_Par_val_left.
-  eapply pure_wp_bind_conseq; first apply He.
-  intros v (a & -> & Hpa).
-  apply pure_wp_widen_pat.
-  unfold continue, discontinue; simpl.
-  eapply pattern_env_mono; first apply Hpa.
-  intros δ Hbindings.
-  eapply pure_wp_mono; first apply Hbindings.
-  - intros ? Hφ. apply pure_wp_ret, pure_wp_ret; auto.
-  - intros exc Hexc. apply pure_wp_throw; auto.
+  simpl_eval_bindings. eapply pure_bind_unary.
+  eapply pure_par_seq.
+  eapply pure_ret_mono. { apply He. } intros a Hpat_a.
+  apply invert_pure_order in Hpat_a.
+  eapply pure_ret_mono. { apply Hpat_a. }
+  intros η' Hpat_η'.
+  apply pure_irrefutably_extend.
+  eapply (pattern_app η η' p ♯a φ ⊥).
+  apply Hpat_η'.
 Qed.
