rocq-osiris/theories/semantics/eval.v
@@ -141,14 +141,6 @@ Definition val_as_loc {E} (v : val) : micro loc E :=
       type_mismatch "location value expected"
   end.
 
-Definition val_as_loc_opt (v : val) : option loc :=
-  match v with
-  | VLoc l =>
-      Some l
-  | _ =>
-      None
-  end.
-
 Definition as_loc {E} (m : micro val E) : micro loc E :=
   v ← m ;
   val_as_loc v.
@@ -285,20 +277,20 @@ Definition as_array (m : microvx) : micro (list loc) exn :=
    through modules, and to have [as_struct] when evaluating module
    expressions. *)
 
-Definition val_as_struct_opt (v : val) : option env :=
-  match v with
-  | VStruct xvs =>
-      Some xvs
-  | _ =>
-      None
-  end.
-
 Definition val_as_struct {E} (v : val) : micro env E :=
   match v with
   | VStruct xvs =>
       ret xvs
   | _ =>
       type_mismatch "structure expected"
+  end.
+
+Definition val_as_struct_opt (v : val) : option env :=
+  match v with
+  | VStruct xvs =>
+      Some xvs
+  | _ =>
+      None
   end.
 
 Definition as_struct {E} (m : micro val E) : micro env E :=
@@ -326,7 +318,8 @@ Fixpoint lookup_name η x : option val :=
   match η with
   | (x', v) :: η =>
       if x =? x' then Some v else lookup_name η x
-  | [] => None
+  | [] =>
+      None
   end.
 
 (* ------------------------------------------------------------------------ *)
@@ -335,7 +328,8 @@ Fixpoint lookup_name η x : option val :=
 
 Fixpoint lookup_path η π : option val :=
   match π with
-  | [] => None
+  | [] =>
+      None
   | [x] =>
       lookup_name η x
   | x1 :: π =>
@@ -411,9 +405,7 @@ Fixpoint lookup_rec_bindings rbs g : option anonfun :=
 
 Section EvalPat.
 
-Local Open Scope stdpp.
-
-Variable eval_pat : env → env → pat → val → option env.
+Variable eval_pat : env → env → pat → val → micro env unit.
 
 (* ------------------------------------------------------------------------ *)
 
@@ -430,19 +422,19 @@ Variable eval_pat : env → env → pat → val → option env.
    left-hand side of a pair can guarantee the safety of a test in the
    right-hand side of this pair. *)
 
-Fixpoint pre_eval_pats (η δ : env) ps vs : option env :=
+Fixpoint pre_eval_pats (η δ : env) ps vs : micro env unit :=
   let eval_pats := pre_eval_pats in
   match ps, vs with
   | [], [] =>
-      Some δ
+      ret δ
   | p::ps, v::vs =>
       δ ← eval_pat η δ p v ;
       δ ← eval_pats η δ ps vs ;
-      Some δ
+      ret δ
   | _::_, [] =>
-      None
+      length_mismatch "longer tuple expected"
   | [], _::_ =>
-      None
+      length_mismatch "shorter tuple expected"
  end.
 
 (* [eval_fpats η δ fps fvs] matches the field-indexed values [fvs] against the
@@ -454,22 +446,18 @@ Fixpoint pre_eval_pats (η δ : env) ps vs : option env :=
 
    A failure occurs if a field is present in [fps] but absent in [fvs]. *)
 
-Fixpoint pre_eval_fpats (η δ : env) fps fvs : option env :=
+Fixpoint pre_eval_fpats (η δ : env) fps fvs : micro env unit :=
   let eval_fpats := pre_eval_fpats in
   match fps with
-  | [] => Some δ
+  | [] => ret δ
   | (f, p) :: fps =>
-      v ← lookup_name fvs f ;
+      v ← of_option (lookup_name fvs f) ;
       δ ← eval_pat η δ p v ;
       δ ← eval_fpats η δ fps fvs ;
-      Some δ
+      ret δ
   end.
 
 End EvalPat.
-
-Section EvalPat.
-
-Local Open Scope stdpp.
 
 (* [eval_pat η δ p v] matches the value [v] against the pattern [p].
 
@@ -490,29 +478,29 @@ Local Open Scope stdpp.
 (* We assume that the pattern [p] is linear: that is, no variable is
    bound twice. This property is enforced by the OCaml type-checker. *)
 
-Local Fixpoint pre_eval_pat η δ p v : option env :=
+Local Fixpoint pre_eval_pat η δ p v : micro env unit :=
   let eval_pat := pre_eval_pat in
   let eval_pats := pre_eval_pats eval_pat in
   let eval_fpats := pre_eval_fpats eval_pat in
   match p, v with
   | PUnsupported, _ =>
-      None
+      unsupported_construct
   | PAny, _ =>
       (* A wildcard pattern always succeeds. *)
-      Some δ
+      ret δ
   | PVar x, _ =>
       (* A variable pattern always succeeds, and causes the environment
          to be extended. *)
-      Some ((x, v) :: δ)
+      ret ((x, v) :: δ)
   | PAlias p x, _ =>
       (* An alias pattern [p as x] is an intersection pattern: the value
          [v] must match both the pattern [p] and the pattern [x]. *)
       δ ← eval_pat η δ p v ;
-      Some ((x, v) :: δ)
+      ret ((x, v) :: δ)
   | POr p1 p2, _ =>
       (* A disjunction pattern [p1 | p2] requires that the value [v]
          match either [p1] or [p2]. *)
-      (eval_pat η δ p1 v) ∪ (eval_pat η δ p2 v)
+      orelse (eval_pat η δ p1 v) (eval_pat η δ p2 v)
   | PTuple ps, VTuple vs =>
       (* A tuple pattern matches a tuple value. *)
       eval_pats η δ ps vs
@@ -520,39 +508,38 @@ Local Fixpoint pre_eval_pat η δ p v : option env :=
       (* A data pattern matches a data value, provided the data constructors
          match. If the data constructors do not match, a meta-level exception
          is raised. *)
-      if c =? c' then eval_pats η δ ps vs else None
+      if c =? c' then eval_pats η δ ps vs else throw ()
   | PXData π ps, VXData l vs =>
       (* A data pattern for an extensible data type matches a data value, provided
          the data constructors correspond to the same location in the environment.
          If the data constructors do not match, a meta-level exception is raised. *)
-      vl' ← (lookup_path η π) ;
-      l' ← val_as_loc_opt vl' ;
-      if (locations.eqb l l') then eval_pats η δ ps vs else None
-  | PRecord fps, VBlock l =>
+      l' ← as_loc (of_option (lookup_path η π)) ;
+      if (locations.eqb l l') then eval_pats η δ ps vs else throw()
+  | PRecord fps, VBlock fvs =>
       (* A record pattern matches a record value. *)
       (* The pattern may have fewer fields than the value. *)
-      None
+      unsupported_construct
   | PInt z, VInt i' =>
       let i := int.repr z in
-      if int.eq i i' then Some δ else None
+      if int.eq i i' then ret δ else throw ()
   | PChar c', VChar c =>
-      if Ascii.eqb c c' then Some δ else None
+      if Ascii.eqb c c' then ret δ else throw ()
   | PString s', VString s =>
-      if s =? s' then Some δ else None
+      if s =? s' then ret δ else throw ()
   | PTuple _, _ =>
-      None
+      type_mismatch "tuple expected"
   | PData _ _, _ =>
-      None
+      type_mismatch "algebraic data expected"
   | PXData _ _, _ =>
-      None
+      type_mismatch "extensible algebraic data expected"
   | PRecord _, _ =>
-      None
+      type_mismatch "record expected"
   | PInt _, _ =>
-      None
+      type_mismatch "integer expected"
   | PChar _, _ =>
-      None
+      type_mismatch "char expected"
   | PString _, _ =>
-      None
+      type_mismatch "string expected"
   end.
 
 Local Definition eval_pat_aux : seal (pre_eval_pat).
@@ -578,7 +565,7 @@ Definition eval_fpats := eval_fpats_aux.(unseal).
 (* [eval_cpat η δ cp o] matches the outcome [o] against
    the computation pattern [cp]. *)
 
-Fixpoint eval_cpat η δ cp o : option env :=
+Fixpoint eval_cpat η δ cp o : micro env unit :=
   match cp, o with
   | CVal p, O3Ret v =>
       (* A value pattern matches a return. *)
@@ -593,14 +580,17 @@ Fixpoint eval_cpat η δ cp o : option env :=
       eval_pat η δ pk (VCont k)
   | COr cp1 cp2, _  =>
       (* A [COr] either matches its first or second branch. *)
-      (eval_cpat η δ cp1 o) ∪ (eval_cpat η δ cp2 o)
+      orelse (eval_cpat η δ cp1 o) (eval_cpat η δ cp2 o)
   | _, _ =>
-      (* If [o] and [cp] don't match, we fail and continue to
-         the next branch.*)
-      None
+      (* If [o] and [cp] don't match, we throw a meta-level exception
+         and continue to the next branch.*)
+      throw()
   end.
 
-End EvalPat.
+(* This variant of [extend] crashes if [p] does not match [v]. *)
+
+Definition irrefutably_extend {E} η δ p v : micro env E :=
+  try (eval_pat η δ p v) ret match_failure.
 
 (* ------------------------------------------------------------------------ *)
 
@@ -634,7 +624,7 @@ Definition call v1 v2 : microvx :=
       let η := δ ++ η in
       (* Look up the entry point [g] in [rbs], yielding an anonymous
          function [a]. *)
-      a ← widen (lookup_rec_bindings rbs g) ;
+      a ← of_option (lookup_rec_bindings rbs g) ;
       (* Then, proceed as in the case of a non-recursive closure. *)
       acall η a v2
    | _ =>
@@ -768,7 +758,7 @@ Implicit Type ηδ : envs.
 
 (* ------------------------------------------------------------------------ *)
 
-Section Coercions.
+Section Coerce.
 
 Local Open Scope stdpp.
 
@@ -807,7 +797,7 @@ Fixpoint coerce (c : coercion) (v : val) : option val :=
       Some (VStruct xvs)
   end.
 
-End Coercions.
+End Coerce.
 
 (* ------------------------------------------------------------------------ *)
 
@@ -943,10 +933,10 @@ Fixpoint pre_eval_mexpr (η : env) (me : mexpr) : microvx :=
       unsupported_construct
   | MPath π =>
       (* A path is looked up in the environment [η]. *)
-      widen (lookup_path η π)
+      of_option (lookup_path η π)
   | MCoercion me c =>
       v ← eval_mexpr η me ;
-      widen (coerce c v)
+      of_option (coerce c v)
   | MStruct items =>
       (* evaluate the structure items, yielding an environment [δ], *)
       '(_, δ) ← eval_sitems (η, []) items ;
@@ -966,21 +956,6 @@ Variable eval : env → expr → microvx.
 
 (* ------------------------------------------------------------------------ *)
 
-(* Evaluate the expression [e], yielding a value [v],
-   and produce an environment fragment [η]. *)
-
-(* A binding is a pair [p = e]. The expressions in the right-hand sides of the
-   bindings [bs] are evaluated in parallel. The values thus obtained are then
-   matched against the patterns in the left-hand sides. The pattern matching
-   process is sequential. *)
-
-(* Every pattern is considered irrefutable, so if a pattern [p] does not
-   match the corresponding value [v], a crash occurs via [widen]. *)
-
-Definition eval_binding η '(Binding p e : binding) : micro env exn :=
-  v ← eval η e;
-  widen (eval_pat η [] p v).
-
 (* [eval_bindings η bs] evaluates the bindings [bs] in the environment [η],
    producing an environment fragment. *)
 
@@ -995,14 +970,12 @@ Fixpoint pre_eval_bindings (η : env) (bs : list binding) : micro env exn :=
   match bs with
   | [] =>
       ret []
-  | b :: bs =>
-      '(η, δ) ← pair_op Strat.let_and_order
-        (eval_binding η b)
-        (* In parallel, evaluate the bindings [bs],
-           yielding an environment fragment [δ]. *)
-        (eval_bindings η bs);
-      (* Finally, concatenate the two environment fragments. *)
-      ret (η ++ δ)
+  | Binding p e :: bs =>
+      (* Evaluate the expression [e], yielding a value [v]. In parallel,
+         evaluate the bindings [bs], yielding an environment fragment [δ]. *)
+      '(v, δ) ← pair_op Strat.let_and_order (eval η e) (eval_bindings η bs);
+       (* Match the value [v] against the pattern [p], extending [δ]. *)
+      irrefutably_extend η δ p v
   end.
 
 (* ------------------------------------------------------------------------ *)
@@ -1077,14 +1050,17 @@ Fixpoint pre_eval_branches η (o : outcome3 val exn) (bs : list branch) : microv
        end)
   | Branch cp e :: bs =>
       (* If we are facing a branch [| cp -> e ]. *)
-      (* We attempt to match the outcome [o] against the pattern [cp]. *)
-      match (eval_cpat η η cp o) with
-      (* In case of success, we evaluate [e] in an environment
-         that has been extended by [eval_cpat]. *)
-      | Some η'  => eval η' e
-      (* If case of failure, we move on to the remaining branches. *)
-      | None => pre_eval_branches η o bs
-      end
+      try2
+        (* We attempt to match the outcome [o] against the pattern [cp]. *)
+        (eval_cpat η η cp o)
+        (λ (oenv : outcome2 env unit),
+          match oenv with
+          (* In case of success, we evaluate [e] in an environment
+             that has been extended by [eval_cpat]. *)
+          | O2Ret η'  => eval η' e
+          (* If case of failure, we move on to the remaining branches. *)
+          | O2Throw () => pre_eval_branches η o bs
+          end)
   end.
 
 
@@ -1125,10 +1101,10 @@ Fixpoint pre_shallow_eval_branches η bs all_bs o :=
            try2 (perform e) (λ o, resume l o)
        end)
   | Branch cp e :: bs =>
-      match (eval_cpat η η cp o) with
-      | Some δ => eval δ e
-      | None => pre_shallow_eval_branches η bs all_bs o
-      end
+      try
+        (eval_cpat η η cp o)
+        (λ δ, eval δ e)
+        (fun tt => pre_shallow_eval_branches η bs all_bs o)
   end.
 
 End Eval.
@@ -1200,7 +1176,7 @@ Fixpoint pre_eval η e {struct e} : microvx :=
       ret (VChar c)
   | EPath π =>
       (* A path [π] is looked up in the environment [η]. *)
-      widen (lookup_path η π)
+      of_option (lookup_path η π)
   | EAnonFun a =>
       (* The creation of a closure captures the environment [η]. *)
       (* This environment is *not* trimmed so as to keep only the variables
@@ -1220,7 +1196,7 @@ Fixpoint pre_eval η e {struct e} : microvx :=
       v ← evals η es ;
       ret (VData c v)
   | EXData π es =>
-      l ← as_loc (widen (lookup_path η π)) ;
+      l ← as_loc (of_option (lookup_path η π)) ;
       v ← evals η es ;
       ret (VXData l v)
   | ERecord t es =>
@@ -1256,14 +1232,14 @@ Fixpoint pre_eval η e {struct e} : microvx :=
       ret (VInt (repr (length ls)))
   | EArrayGet e1 e2 =>
       '(ls, i) ← par (as_array (eval η e1)) (as_int (eval η e2)) ;
-      match ls !! (signed i) with
+      match ls !! signed i with
       | Some l => load l
       | None => crash "index out of bounds"
       end
   | EArraySet e1 e2 e3 =>
       '(ls, (i, v)) ← par (as_array (eval η e1))
                        (par (as_int (eval η e2)) (eval η e3));
-        match ls !! (signed i) with
+        match ls !! signed i with
         | Some l => store l v
         | None => crash "index out of bounds"
         end
@@ -1664,7 +1640,8 @@ Ltac simpl_eval_pats :=
   || fail "Unable to simplify application of eval_pats".
 
 Ltac simpl_eval_pat :=
-  (unfold eval_pat;
+  (unfold irrefutably_extend;
+   unfold eval_pat;
    rewrite seal_eq;
    (progress simpl pre_eval_pat);
    rewrite ?fold_pre_eval_pat, ?fold_pre_eval_pats)
@@ -1674,7 +1651,7 @@ Ltac unfold_all :=
   unfold eval, evals, evalfs,
     eval_branches, shallow_eval_branches,
     eval_bindings, eval_sitem, eval_sitems, eval_mexpr,
-    eval_pats, eval_pat;
+    eval_pats, irrefutably_extend, eval_pat;
   rewrite ?seal_eq.
 
 Ltac fold_all :=
