rocq-osiris/theories/semantics/micro.v
@@ -380,9 +380,15 @@ Definition orelse {A E E'} (m1 : micro A E') (m2 : micro A E) : micro A E :=
    must be converted to the type [micro _ E]. The coercion [widen]
    is used for this purpose. *)
 
-Definition widen {A E} (m : option A) : micro A E :=
-  match m with
-  | Some a => ret a
+Definition widen {A E} (m : micro A void) : micro A E :=
+  try m ret elim_void.
+
+(* [of_option o] converts an option value [o] into a computation: [Some v]
+   becomes [ret v], and [None] becomes [Crash]. *)
+
+Definition of_option {A E} (o : option A) : micro A E :=
+  match o with
+  | Some v => ret v
   | None => Crash
   end.
 
