examples/proofs/localstate.v
@@ -132,8 +132,8 @@ Section verification.
 
   Lemma localstate_run_spec :
     ∀ η,
-      ⌜ lookup_name η "Get" = Some #rl ⌝ -∗
-      ⌜ lookup_name η "Set" = Some #wl ⌝ -∗
+      ⌜ lookup_name η "Get" = ret (VLoc rl) ⌝ -∗
+      ⌜ lookup_name η "Set" = ret (VLoc wl) ⌝ -∗
       ⌜ address rl ≠ address wl ⌝ -∗
       imp eval η (EAnonFun __fun7)
         {{ λ run,  □ iSpec τ[ state;val] run run_spec }}.
@@ -239,7 +239,7 @@ Section verification.
 
   Lemma module_proof (Q : val -> iProp Σ) :
     ⊢ imp (eval_mexpr dummy_env __main)
-      {{ λ η, ∃ run, ⌜lookup_name η "run" = Some run⌝ ∗
+      {{ λ η, ∃ run, ⌜lookup_name η "run" = ret run⌝ ∗
                      □ iSpec τ[state; val] run run_spec }}.
   Proof.
     iApply imp_module.
@@ -247,7 +247,7 @@ Section verification.
 
     (* [open Effect] *)
     { iApply (imp_sitem_open).
-      { simpl_eval_mexpr.
+      { simpl_eval_mexpr. iApply imp_widen.
         iApply imp_ret; first encode.
         instantiate (1 := (λ δ, ⌜δ = [_]⌝)%I). done. }
       iIntros (? ->) "/=".
@@ -257,7 +257,7 @@ Section verification.
     (* [open Effect.Deep] *)
     iApply imp_sitems_cons.
     { iApply (imp_sitem_open).
-      { simpl_eval_mexpr.
+      { simpl_eval_mexpr. iApply imp_widen.
         iApply imp_ret; first encode.
         instantiate (1 := (λ δ, ⌜δ = []⌝)%I). done. }
       iIntros (? ->) "/=".
