rocq-osiris/theories/lang/notations.v
@@ -251,6 +251,20 @@ Goal (trivial
 Abort.
 
 (* -------------------------------------------------------------------------- *)
+(* Loops and conditionals. *)
+
+Notation "e1 ;; e2" :=
+  (ESeq e1 e2)
+    (at level 100, e2 at level 200,
+      format "'[' '[hv' '[' e1 ']' ;; ']' '/' e2 ']'").
+
+Goal (trivial
+        (ESeq
+         (EApp (EPath ["f"]) (EPath ["x"]))
+         (EAssert (EOpEq (EPath ["x"]) (EInt 2))))).
+Abort.
+
+(* -------------------------------------------------------------------------- *)
 (* Pattern matching. *)
 
 Notation "'EMatch' '(' x ')' []" :=
