rocq-osiris/theories/program_logic/pure/expr_rules.v
@@ -11,13 +11,13 @@ From osiris.program_logic.pure Require Import
 
 (* EPath (x : path) *)
 
-Lemma pure_eval_path `{Encode A} η π (ψ : A -> Prop) (ζ : exn -> Prop) :
-  (∃ a, lookup_path η π = Some #a ∧ ψ a) ->
-  pure (eval η (EPath π)) ψ ζ.
+Lemma pure_eval_path `{Encode A} η π (φ : A -> Prop) (ζ : exn -> Prop) a :
+  lookup_path η π = Some #a →
+  φ a →
+  pure (eval η (EPath π)) φ ζ.
 Proof.
-  simpl_eval. firstorder. apply pure_wp_widen.
-  exists #x. split; first done. unfold returns.
-  eauto.
+  simpl_eval. intros -> Hφ.
+  eapply pure_ret; eauto.
 Qed.
 
 (* -------------------------------------------------------------------------- *)
@@ -1005,8 +1005,9 @@ Lemma pure_eval_let `{Encode A} η bs e (φ : A → Prop) ψ :
 Proof.
   intros Hbs.
   simpl_eval.
-  eapply pure_wp_bind.
-  eapply (pure_wp_mono _ Hbs); eauto.
+  eapply pure_bind_unary.
+  eapply pure_ret_mono; [ apply Hbs | ].
+  intros η' He. apply He.
 Qed.
 
 Lemma pure_eval_let1 `{Encode A, Encode B} η p e1 e (φ : B → Prop) ψ :
@@ -1016,11 +1017,10 @@ Proof.
   intros He1.
   eapply pure_eval_let.
   eapply bindings_cons. apply He1.
-  intros a Hpat. apply Hpat.
   eapply bindings_nil. apply eq_refl.
   intros a η'.
   intros Hpat <-.
-  rewrite app_nil_r. apply Hpat.
+  apply Hpat.
 Qed.
 
 Lemma pure_eval_let1_conseq `{Encode A, Encode B} η p e1 e (φ1 : A → Prop) (φ : B → Prop) ψ :
@@ -1062,15 +1062,11 @@ Lemma pure_eval_let1var `{Encode A1, Encode B} η x e1 e
 Proof.
   intros He1 He.
   eapply pure_eval_let.
-  eapply bindings_cons.
-  - apply He1.
-  - intros a Hφ1. apply pat_PVar.
-    instantiate (1:= λ η, ∃ a, η = [(x, #a)] ∧ φ1 a).
-    exists a. auto.
-  - apply bindings_nil. apply eq_refl.
-  - intros a η' (? & -> & Hφ1) <-.
-    rewrite app_nil_r.
-    by apply He.
+  eapply bindings_cons. apply He1.
+  apply bindings_nil. apply eq_refl.
+  intros a η' Hφ1 <-.
+  apply pat_PVar.
+  by apply He.
 Qed.
 
 Lemma pure_eval_let_simple `{Encode A1, Encode B} η x e1 e
@@ -1085,38 +1081,43 @@ Proof.
 Qed.
 
 Lemma pure_eval_let_pair `{Encode A1, Encode A2} `{Encode X}
-  p1 p2 e1 e2 η φ P (ψ : X -> Prop) ζ :
-  pure (eval η e1) (λ '((v1, v2) : A1 * A2), φ (v1, v2)) ζ →
-  (∀ v1 v2, φ (v1, v2) →
-            pattern η [] p1 #v1 (λ δ, pattern η δ p2 #v2 (P v1 v2) False) False) →
-  (∀ v1 v2 δ, φ (v1, v2) → P v1 v2 δ → pure (eval (δ ++ η) e2) ψ ζ) →
+  p1 p2 e1 e2 η (ψ : X -> Prop) ζ :
+  pure (eval η e1) (λ '((v1, v2) : A1 * A2),
+      pure (
+          δ ← irrefutably_extend η [] p1 #v1;
+          θ ← irrefutably_extend η δ p2 #v2;
+          eval (θ ++ η) e2
+        ) ψ ζ) ζ ->
   pure (eval η (ELet1 (PPair p1 p2) e1 e2)) ψ ζ.
 Proof.
-  intros He1 Hpat He2. simpl_eval.
-  eapply pure_bind. eapply (pure_bind (A1:= env * env)).
-  { instantiate (1 := λ '(δ, l), l = [] ∧ pure (eval (δ ++ η) e2) ψ ζ).
-    Set Printing Implicit. Unset Printing Notations.
-    eapply pure_par'.
-    - instantiate (1:= λ δ, (∃ v1 v2, φ (v1, v2) ∧ P v1 v2 δ)).
-      eapply pure_bind. apply He1.
-      intros [??] Hφ.
-      eapply pure_widen_pat.
-      eapply pattern_mono_exn.
-      eapply pat_PPair; try reflexivity.
-      eapply pattern_env_mono.
-      apply Hpat, Hφ. intros δ Hpat2. simpl in Hpat2.
-      eapply pattern_env_mono.
-      apply Hpat2. intros δ' HP. eauto.
-      tauto.
-    - eapply pure_ret; first encode. apply eq_refl.
-    - intros η' δ' (v1 & v2 & Hφ & HP) ->.
-      split; first reflexivity.
-      eauto. }
-  intros (δ & ?) (-> & He2').
-  eapply (pure_ret _ _ _ δ). simpl. by rewrite app_nil_r.
-  apply He2'.
-  intros δ Hδ.
-  rewrite bind_ret. apply Hδ.
+  intros He1. simpl_eval.
+  (* This proof is a long rewriting sequence, which makes some sense as it is
+     not the standard method to prove a let binding, but rather a way to reduce the
+     wp of a parallel pair to ordered wps of two binds with error handling *)
+  do 2 eapply pure_bind_unary.
+  eapply pure_par. apply He1. eapply pure_ret; [ encode | apply eq_refl ].
+  intros (a1, a2) ? He2 <-. simpl.
+  unfold widen, irrefutably_extend in *.
+  simpl_eval_pat.
+  rewrite !bind_as_try, !try_try in *.
+  apply pure_wp_try2.
+  apply invert_pure_wp_try2 in He2.
+  eapply pure_wp_mono. apply He2. all: clear He2.
+  - unfold continue. simpl.
+    intros η'.
+    rewrite try_ret.
+    repeat rewrite ?bind_as_try, ?try_try, ?try_ret in *.
+    intros Hpure_wp.
+    apply invert_pure_wp_try2 in Hpure_wp.
+    apply pure_wp_try2.
+    apply (pure_wp_mono _ Hpure_wp); clear Hpure_wp.
+    + intros θ Hpure_wp.
+      unfold continue, glue2 in *.
+      repeat rewrite ?bind_as_try, ?try_try, ?try_ret in *.
+      apply pure_wp_ret.
+      exists θ; auto.
+    + unfold match_failure. rewrite try_crash. intros. edestruct @invert_pure_wp_crash; eauto.
+  - unfold match_failure. rewrite try_crash. intros. edestruct @invert_pure_wp_crash; eauto.
 Qed.
 
 (* -------------------------------------------------------------------------- *)
@@ -1334,8 +1335,12 @@ Lemma branches_cons_unary `{Encode A} η o cp e bs (φ : A -> Prop) ψ :
   branches η o (Branch cp e :: bs) φ ψ.
 Proof.
   unfold branches.
-  intros Hcpat; simpl_eval_branches. unfold cpattern in Hcpat.
-  destruct (eval_cpat η η cp o); auto.
+  intros; simpl_eval_branches.
+  eapply pure_try2. apply H0.
+  - intros η' He.
+    unfold continue. apply He.
+  - intros [] Hbranches.
+    unfold discontinue. apply Hbranches.
 Qed.
 
 Lemma branches_cons `{Encode A} η o cp e bs (φ : A -> Prop) ψ' ψ :
@@ -1345,7 +1350,8 @@ Lemma branches_cons `{Encode A} η o cp e bs (φ : A -> Prop) ψ' ψ :
 Proof.
   intros.
   apply branches_cons_unary.
-  eapply cpattern_mono; eauto.
+
+  eapply pure_wp_mono; eauto.
 Qed.
 
 (* Not matching a value is an error. *)
